moved the glueing definitions to end to end file

hol/bdd_end_to_endScript.sml
@@ -30,10 +30,26 @@ open policy_specTheory;
 open tables_specTheory;
 
 
+open policy_arith_to_varTheory;
+open table_var_to_arithTheory;
+open table_arith_to_intervalTheory;
+
+
+open bdd_auxTheory;
+open table_bs_propertiesTheory;
+
+
 
      
      
 val _ = new_theory "bdd_end_to_end";
+
+
+
+(******************************************)
+(*        var policy to var table         *)
+(*            glue of theorems            *)
+(******************************************)
 
 
         
@@ -832,12 +848,418 @@ QED
 
 
 
+(******************************************
+   
+arith policy to interval table requirement for gluing all assumtions of equiality theorems:                       
+       cond1 ==> (arith_policy =  var_policy)
+       cond2 ==> (var_policy = var_table)    
+        cond1 /\ cond3 ==> (var_table = interval_table)                      
 
+cond1 is: 
+(∀var atom. 
+       ALOOKUP m_e var = SOME atom ⇒ 
+       ALOOKUP m_v var = eval_arithm_atom packet_input atom) ∧
+    (convert_arith_to_var_policy arith_policy m_e = SOME var_policy)
+
+cond2 is:
+mv_dom_vars mv order
+
+cond3 is:
+(∀var. lookup_is_some mv var ⇔ lookup_is_some me var)
+******************************************)
+
+
+(* definitions and proofs for cond1 *)
+
+Definition mv_from_me_and_packet_def:
+  mv_from_me_and_packet me packet_input =
+  MAP (\(x,arith_atom). 
+        case eval_arithm_atom packet_input arith_atom of
+          NONE => NONE
+        | SOME v => SOME (x, v)
+      ) me
+End
+
+
+
+Definition create_mv_def:
+  create_mv me packet_input =
+  let all = mv_from_me_and_packet me packet_input in
+    let filtered = FILTER IS_SOME all in
+      MAP THE filtered
+End
+                                     
+ 
+Definition every_lval_in_me_in_type_def:
+  every_lval_in_me_in_type pd_type me =
+   EVERY (\(x,atom).  case (get_lval_from_arith atom) of
+                      | is_lval lval => (case resolve_lval_type pd_type lval of
+                                         | SOME (type_length n) => T
+                                         | _ => F ) 
+                      | _ => T) me                      
+End
+
+
+
+Definition ops_in_me_length_format_def:
+  ops_in_me_length_format pd_type me =
+  EVERY (\(x,atom).  case atom of
+                     | a_True => T
+                     | a_False => F           
+                     | arithm_ge lval m => (case resolve_lval_type pd_type lval of
+                                            | SOME (type_length n) => (n = SND m) 
+                                            | _ => F )
+                     | arithm_le lval m => (case resolve_lval_type pd_type lval of
+                                            | SOME (type_length n) => (n = SND m) 
+                                            | _ => F ) 
+        ) me                      
+End
+     
+
+     
+    
+Theorem lval_in_me_distinct_imp_cond1:
+∀ me pd_type packet_input .
+  ALL_DISTINCT (MAP FST me) ∧
+  every_lval_in_me_in_type pd_type me ⇒
+  (∀var atom.
+     ALOOKUP me var = SOME atom ⇒
+     ALOOKUP (create_mv me packet_input) var = eval_arithm_atom packet_input atom)
+Proof
+Induct >>
+rpt strip_tac >>
+gvs[create_mv_def] >>                 
+rw[mv_from_me_and_packet_def] >|[
+    PairCases_on ‘h’ >> gvs[] >>
+    rpt (BasicProvers.FULL_CASE_TAC >> gvs[]) >>
+    gvs[every_lval_in_me_in_type_def] >>
+    res_tac >>
+    gvs[mv_from_me_and_packet_def]
+    ,
+    PairCases_on ‘h’ >> gvs[] >>
+    rpt (BasicProvers.FULL_CASE_TAC >> gvs[]) >|[
+        simp[ALOOKUP_NONE] >>
+        gvs[MEM_MAP] >>
+        rpt strip_tac >>
+        gvs[MEM_FILTER] >>
+        gvs[MEM_MAP] >>
+        PairCases_on ‘y’ >> gvs[] >>
+        rpt (BasicProvers.FULL_CASE_TAC >> gvs[])
+                           
+        ,
+        gvs[every_lval_in_me_in_type_def] >>
+        res_tac >>
+        gvs[mv_from_me_and_packet_def]    
+      ]
+  ]
+QED
+    
+
+
+
+(* definitions and proofs for cond2 *)
+
+
+  
+Definition mv_dom_vars_exec_def:
+  mv_dom_vars_exec mv vars =
+  EVERY (\x. ALOOKUP mv x ≠ NONE) vars
+End
+
+Theorem lookup_is_some_not_none_eq:
+  ∀ mv x.
+    lookup_is_some mv x ⇔ ALOOKUP mv x ≠ NONE
+Proof
+  Induct >>
+  gvs[lookup_is_some_def] >>
+  rpt strip_tac >>
+  EQ_TAC >>
+  rpt strip_tac >>
+  gvs[] >>
+  Cases_on ‘ALOOKUP (h::mv) x’ >> gvs[]
+QED                  
+                                 
+        
+Theorem mv_dom_vars_exec_eq:
+  ∀ mv vars.
+    mv_dom_vars mv vars = mv_dom_vars_exec mv vars
+Proof
+  rw[mv_dom_vars_def, mv_dom_vars_exec_def] >>
+  gvs[EVERY_MEM, lookup_is_some_not_none_eq]
+QED
+
+
+
+Definition in_order_then_in_me_def:
+  in_order_then_in_me order me =
+  EVERY (\x. ALOOKUP me x ≠ NONE) order
+End
+
+
+
+Theorem wf_format_imp_cond2:
+  ∀ me pd_type order.
+    ∀ packet_input.
+      in_order_then_in_me order me ∧
+      ops_in_me_length_format pd_type me ∧
+      wf_packet pd_type packet_input ∧
+      ALL_DISTINCT (MAP FST me) ∧
+      every_lval_in_me_in_type pd_type me ⇒
+      mv_dom_vars (create_mv me packet_input) order
+Proof
+  rw[in_order_then_in_me_def] >>
+  gvs[mv_dom_vars_exec_eq] >>
+  gvs[mv_dom_vars_exec_def] >>
+  gvs[EVERY_MEM] >>
+  rpt strip_tac >>
+  res_tac >>
+  
+  
+  Cases_on ‘ALOOKUP me x’ >> gvs[] >>
+  imp_res_tac MEM_ALOOKUP_DISTINCT >>
+  
+  gvs[every_lval_in_me_in_type_def] >>
+  gvs[EVERY_MEM] >>
+  
+  res_tac >>
+  gvs[create_mv_def] >>
+  gvs[mv_from_me_and_packet_def] >>         
+  gvs[ALOOKUP_NONE] >>
+  gvs[MEM_MAP] >>
+  gvs[MEM_FILTER] >>
+  gvs[MEM_MAP] >>
+  
+  first_x_assum (strip_assume_tac o (Q.SPECL [‘(x,THE (eval_arithm_atom packet_input x'))’])) >> gvs[] >>
+  first_x_assum (strip_assume_tac o (Q.SPECL [‘SOME (x,THE (eval_arithm_atom packet_input x'))’])) >> gvs[] >>
+  first_x_assum (strip_assume_tac o (Q.SPECL [‘(x,x')’])) >> gvs[] >>
+  
+  rpt (BasicProvers.FULL_CASE_TAC >> gvs[]) >>
+  
+  Cases_on ‘x'’ >> 
+  gvs[eval_arithm_atom_def] >>
+  
+  rpt (BasicProvers.FULL_CASE_TAC >> gvs[]) >>
+  (* le and ge same proof *)
+  (
+  (* first and third subgoals *)
+  res_tac >>
+  fs[get_lval_from_arith_def] >>
+  rpt (BasicProvers.FULL_CASE_TAC >> gvs[]) >>
+  gvs[wf_packet_def] >>
+  res_tac >> gvs[] >>
+  
+  (* reach here only for second subgoal *)
+  
+  PairCases_on ‘bs’ >>
+  PairCases_on ‘y’ >>
+  PairCases_on ‘y'’ >>
+  gvs[] >>
+  
+  imp_res_tac MEM_ALOOKUP_DISTINCT >>
+  gvs[] >>
+  
+  gvs[ops_in_me_length_format_def] >>
+  gvs[EVERY_MEM] >>
+  res_tac >>
+  fs[] >>
+  
+  gvs[] >>
+  
+  PairCases_on ‘p’ >> gvs[] >>
+  imp_res_tac last_edge_of_binpred_neg >> gvs[]
+  )
+QED
 
 
     
+(* definitions and proofs for cond3 *)
 
  
+
+
+
+Theorem create_mv_all_distinct:
+  ∀ me packet_input.
+    ALL_DISTINCT (MAP FST me) ⇒ ALL_DISTINCT (MAP FST (create_mv me packet_input))
+Proof
+  Induct >>
+  gvs[create_mv_def] >>
+  gvs[mv_from_me_and_packet_def] >>   
+  rpt strip_tac >>
+  
+  PairCases_on ‘h’ >> gvs[] >>
+  rpt (BasicProvers.FULL_CASE_TAC >> gvs[]) >>
+  
+  gvs[MEM_MAP, MEM_FILTER] >>
+  rpt strip_tac >>
+  Cases_on ‘y'’ >> gvs[] >>
+  rpt strip_tac >>
+  PairCases_on ‘y’ >> gvs[] >>
+  rpt (BasicProvers.FULL_CASE_TAC >> gvs[])
+QED
+                                              
+
+                                        
+Theorem create_mv_normalization:
+  ∀ h me packet_input.
+  create_mv (h::me) packet_input = (create_mv [h] packet_input)++(create_mv me packet_input)
+Proof
+  rw[create_mv_def] >>
+  gvs[mv_from_me_and_packet_def] >>
+  rpt (BasicProvers.FULL_CASE_TAC >> gvs[])
+QED
+
+
+Theorem ops_in_me_length_format_normalization:
+  ∀ h me pd_type.
+    ops_in_me_length_format pd_type (h::me) = (ops_in_me_length_format pd_type [h] ∧
+                                               ops_in_me_length_format pd_type me)
+Proof
+  rw[ops_in_me_length_format_def]
+QED
+
+
+        
+Theorem every_lval_in_me_in_type_normalization:
+  ∀ h me pd_type.
+    every_lval_in_me_in_type pd_type (h::me) = (every_lval_in_me_in_type pd_type [h] ∧
+                                                every_lval_in_me_in_type pd_type me )
+Proof
+  rw[every_lval_in_me_in_type_def]
+QED
+
+        
+                               
+Theorem if_in_create_mv_then_in_me:                                  
+  ∀ me var y.
+    ∀ packet_input.
+      ALL_DISTINCT (MAP FST me) ∧
+      ALOOKUP (create_mv me packet_input) var = SOME y ⇒
+      ∃y'. ALOOKUP me var = SOME y'
+Proof
+  Induct >>
+  rw[] >-
+   gvs[create_mv_def, mv_from_me_and_packet_def] >>
+  
+  imp_res_tac create_mv_all_distinct >>
+  first_x_assum (strip_assume_tac o (Q.SPECL [‘packet_input’])) >> 
+  
+  gvs[Once create_mv_normalization] >>
+  gvs[ALOOKUP_APPEND] >>
+  rpt (BasicProvers.FULL_CASE_TAC >> gvs[]) >|[
+    res_tac >>
+    PairCases_on ‘h’ >> gvs[] >>
+    BasicProvers.FULL_CASE_TAC >> gvs[]
+    ,
+    PairCases_on ‘h’ >> gvs[] >>
+    BasicProvers.FULL_CASE_TAC >> gvs[] >>
+    gvs[create_mv_def, mv_from_me_and_packet_def] >>
+    rpt (BasicProvers.FULL_CASE_TAC >> gvs[])
+  ]
+QED
+
+
+
+        
+Theorem wf_format_and_fail_create_single:
+  ∀ pd_type h var.
+    ∀ packet_input.
+      ops_in_me_length_format pd_type [h] ∧
+      wf_packet pd_type packet_input ∧
+      every_lval_in_me_in_type pd_type [h]  ∧
+      wf_packet pd_type packet_input ∧
+      ALOOKUP (create_mv [h] packet_input) var = NONE ⇒
+      FST h ≠ var
+Proof
+  
+  rw[create_mv_def] >>
+  gvs[mv_from_me_and_packet_def] >>
+  PairCases_on ‘h’ >> gvs[] >>
+  rpt (BasicProvers.FULL_CASE_TAC >> gvs[]) >>
+  gvs[every_lval_in_me_in_type_def] >>
+  
+  
+  Cases_on ‘h1’ >>
+  gvs[eval_arithm_atom_def] >>
+  rpt (BasicProvers.FULL_CASE_TAC >> gvs[]) >>
+  
+  
+  gvs[get_lval_from_arith_def] >>
+  
+  gvs[wf_packet_def] >>      
+  res_tac >>
+  gvs[] >>
+  
+  gvs[ops_in_me_length_format_def] >>
+  PairCases_on ‘p’ >> gvs[] >>
+  PairCases_on ‘bs’ >> gvs[] >>
+  imp_res_tac last_edge_of_binpred_neg >> gvs[]
+QED
+
+
+
+
+
+Theorem if_in_me_then_in_create_mv:                                  
+  ∀ me pd_type var y.
+    ∀ packet_input.
+      ops_in_me_length_format pd_type me ∧
+      wf_packet pd_type packet_input ∧
+      ALL_DISTINCT (MAP FST me) ∧
+      every_lval_in_me_in_type pd_type me ∧
+      ALOOKUP me var = SOME y
+      ⇒
+      ∃y'. ALOOKUP (create_mv me packet_input) var = SOME y'
+Proof
+
+  Induct >-
+   rw[] >>
+  rpt strip_tac >>
+  
+  imp_res_tac create_mv_all_distinct >>
+  first_x_assum (strip_assume_tac o (Q.SPECL [‘packet_input’])) >> 
+  
+  gvs[Once create_mv_normalization] >>
+  simp[Once create_mv_normalization] >>
+  
+  gvs[ALOOKUP_APPEND] >>
+  rpt (BasicProvers.FULL_CASE_TAC >> gvs[]) >>
+  
+  rgs[Once ops_in_me_length_format_normalization] >>
+  rgs[Once every_lval_in_me_in_type_normalization] >>
+  
+  res_tac >>
+  
+  imp_res_tac wf_format_and_fail_create_single >>
+  PairCases_on ‘h’ >> gvs[] >>
+  res_tac >> gvs[]
+QED
+              
+
+
+
+Theorem wf_format_imp_cond3:                                        
+  ∀ me pd_type.
+    ∀ packet_input.
+      ops_in_me_length_format pd_type me ∧
+      wf_packet pd_type packet_input ∧
+      ALL_DISTINCT (MAP FST me) ∧
+      every_lval_in_me_in_type pd_type me ⇒
+      (∀var. lookup_is_some (create_mv me packet_input) var ⇔
+               lookup_is_some me var)
+Proof
+  rw[lookup_is_some_def] >>
+  EQ_TAC >> strip_tac >|[
+    imp_res_tac if_in_create_mv_then_in_me >> gvs[]
+    ,
+    imp_res_tac if_in_me_then_in_create_mv >> gvs[]
+  ]
+QED
+
+
+
+
+
 
 val _ = export_theory ();
 
